Rework (extend) ax_ctxt and ax_int
In two ways:
1. Accept an arbitrary context (and interpretation) on which to build
   (rather than forcing hol_ctxt/hol_model)
2. Accept some terms to be added as NewAxioms on top of the context.

The good_context theorem has been reproved. But it has additional
assumptions now (about the incoming context and interpretation on which
we are building), and the automation has not been updated to prove
those.

reflectionScript.sml
@@ -2632,22 +2632,25 @@ val NewConsts_ctxt_def = Define`
   NewConsts_ctxt = MAP (λ(name,type,(cs:('U list # 'U) list)). NewConst name type)`;
 
 val ax_ctxt_def = Define`
-  ax_ctxt tys tms =
+  ax_ctxt ctxt ths tys tms =
+    MAP NewAxiom ths ++
     NewConsts_ctxt tms ++
     NewTypes_ctxt tys ++
-    hol_ctxt`;
+    ctxt`;
 
 (* assumptions on tys and tms: *)
-val [tys,tms] = ax_ctxt_def |> INST_TYPE[alpha|->universe_ty,beta|->universe_ty]
-                |> SPEC_ALL |> concl |> lhs |> strip_comb |> #2
-val distinct_tys = ``ALL_DISTINCT (MAP FST (type_list (NewTypes_ctxt ^tys ++ hol_ctxt)))``
-val distinct_tms = ``ALL_DISTINCT (MAP FST (const_list (NewConsts_ctxt ^tms ++ hol_ctxt)))``
+val [ctxt,ths,tys,tms] =
+  ax_ctxt_def |> INST_TYPE[alpha|->universe_ty,beta|->universe_ty]
+  |> SPEC_ALL |> concl |> lhs |> strip_comb |> #2
+val distinct_tys = ``ALL_DISTINCT (MAP FST (type_list (NewTypes_ctxt ^tys ++ ^ctxt)))``
+val distinct_tms = ``ALL_DISTINCT (MAP FST (const_list (NewConsts_ctxt ^tms ++ ^ctxt)))``
 val disjoint_tys = ``EVERY ((ALL_DISTINCT o MAP FST) o SND o SND) ^tys``
 val disjoint_tms = ``EVERY ((ALL_DISTINCT o MAP FST) o SND o SND) ^tms``
 val inhabited_tys = ``EVERY (EVERY (inhabited o SND) o SND o SND) ^tys``
-val types_ok = ``EVERY (type_ok (tysof (NewTypes_ctxt ^tys ++ hol_ctxt)) o FST o SND) ^tms``
+val types_ok = ``EVERY (type_ok (tysof (NewTypes_ctxt ^tys ++ ^ctxt)) o FST o SND) ^tms``
 val _ = overload_on("intype",``λδ ty (args,u).
         u <: typesem δ ((K boolset) =++ ZIP (mlstring_sort (tyvars ty),args)) ty``);
+val props_ok = ``EVERY (λp. term_ok (sigof (NewConsts_ctxt ^tms ++ NewTypes_ctxt ^tys ++ ^ctxt)) p ∧ typeof p = Bool) ^ths``
 (*  - ... constrained constant values in appropriate typesem ...  *)
 
 val ALL_DISTINCT_MAP_FST_type_list_NewTypes_ctxt = Q.store_thm("ALL_DISTINCT_MAP_FST_type_list_NewTypes_ctxt",
@@ -2680,11 +2683,11 @@ val ALOOKUP_const_list_NewConsts_ctxt = Q.store_thm("ALOOKUP_const_list_NewConst
   rw[NewConsts_ctxt_def,MAP_MAP_o,o_DEF,UNCURRY,FLAT_MAP_SING]
   \\ rw[ALOOKUP_MAP_gen,Once LAMBDA_PROD,ETA_AX]);
 
-val NewTypes_ctxt_extends_hol_ctxt = Q.store_thm("NewTypes_ctxt_extends_hol_ctxt",
+val NewTypes_ctxt_extends = Q.store_thm("NewTypes_ctxt_extends",
   `∀tys.
    ^distinct_tys
    ⇒
-   NewTypes_ctxt tys ++ hol_ctxt extends hol_ctxt`,
+   NewTypes_ctxt tys ++ ctxt extends ctxt`,
   simp[NewTypes_ctxt_def]
   \\ Induct \\ simp[]
   >- metis_tac[RTC_REFL,extends_def]
@@ -2696,8 +2699,8 @@ val NewTypes_ctxt_extends_hol_ctxt = Q.store_thm("NewTypes_ctxt_extends_hol_ctxt
   \\ simp[Once updates_cases]);
 
 val NewConsts_ctxt_extends = Q.store_thm("NewConsts_ctxt_extends",
-  `∀tms ctxt.
-   ALL_DISTINCT (MAP FST (const_list (NewConsts_ctxt tms ++ ctxt))) ∧
+  `∀tms.
+   ^distinct_tms ∧
    EVERY (type_ok (tysof ctxt) o FST o SND) tms
    ⇒
    NewConsts_ctxt tms ++ ctxt extends ctxt`,
@@ -2716,32 +2719,73 @@ val NewConsts_ctxt_extends = Q.store_thm("NewConsts_ctxt_extends",
   \\ match_mp_tac SUBMAP_FUNION
   \\ simp[IN_DISJOINT,MEM_FLAT,MEM_MAP,FORALL_PROD,PULL_EXISTS]);
 
+val NewAxioms_ctxt_extends = Q.store_thm("NewAxioms_ctxt_extends",
+  `∀ths. EVERY (λp. term_ok (sigof ctxt) p ∧ typeof p = Bool) ths ⇒
+   MAP NewAxiom ths ++ ctxt extends ctxt`,
+  Induct \\ simp[]
+  >- metis_tac[RTC_REFL,extends_def]
+  \\ fs[] \\ rw[]
+  \\ simp[extends_def]
+  \\ simp[Once RTC_CASES1]
+  \\ simp[GSYM extends_def]
+  \\ simp[Once updates_cases]
+  \\ imp_res_tac term_ok_welltyped
+  \\ conj_tac >- metis_tac[WELLTYPED]
+  \\ match_mp_tac term_ok_extend
+  \\ first_assum(part_match_exists_tac (last o strip_conj) o concl)
+  \\ simp[]
+  \\ conj_tac
+  \\ match_mp_tac SUBMAP_FUNION
+  \\ simp[IN_DISJOINT,MEM_FLAT,MEM_MAP,FORALL_PROD,PULL_EXISTS]);
+
 val const_list_NewTypes_ctxt = Q.store_thm("const_list_NewTypes_ctxt[simp]",
   `const_list (NewTypes_ctxt tys) = []`,
   rw[NewTypes_ctxt_def,MAP_FLAT,MAP_MAP_o,o_DEF,UNCURRY,FLAT_EQ_NIL,EVERY_MAP]);
+
+val type_list_NewConsts_ctxt = Q.store_thm("type_list_NewConsts_ctxt[simp]",
+  `type_list (NewConsts_ctxt tys) = []`,
+  rw[NewConsts_ctxt_def,MAP_FLAT,MAP_MAP_o,o_DEF,UNCURRY,FLAT_EQ_NIL,EVERY_MAP]);
+
+val type_list_NewAxioms_ctxt = Q.store_thm("type_list_NewAxioms_ctxt[simp]",
+  `type_list (MAP NewAxiom ths) = []`,
+  rw[MAP_FLAT,MAP_MAP_o,o_DEF,UNCURRY,FLAT_EQ_NIL,EVERY_MAP]);
 
 val tysof_NewConsts_ctxt = Q.store_thm("tysof_NewConsts_ctxt[simp]",
   `tysof (NewConsts_ctxt tms ++ ctxt) = tysof ctxt`,
   rw[NewConsts_ctxt_def,MAP_MAP_o,o_DEF,UNCURRY,FLAT_MAP_NIL]);
 
-val ax_ctxt_extends_hol_ctxt = Q.store_thm("ax_ctxt_extends_hol_ctxt",
+val tysof_NewAxioms_ctxt = Q.store_thm("tysof_NewAxioms_ctxt[simp]",
+  `tysof (MAP NewAxiom ths ++ ctxt) = tysof ctxt`,
+  rw[MAP_MAP_o,o_DEF,UNCURRY,FLAT_MAP_NIL]);
+
+val tmsof_NewAxioms_ctxt = Q.store_thm("tmsof_NewAxioms_ctxt[simp]",
+  `tmsof (MAP NewAxiom ths ++ ctxt) = tmsof ctxt`,
+  rw[MAP_MAP_o,o_DEF,UNCURRY,FLAT_MAP_NIL]);
+
+val ax_ctxt_extends_ctxt = Q.store_thm("ax_ctxt_extends_ctxt",
   `^distinct_tys ∧
    ^distinct_tms ∧
-   ^types_ok
+   ^types_ok ∧
+   ^props_ok
    ⇒
-   ax_ctxt tys tms extends hol_ctxt`,
+   ax_ctxt ctxt ths tys tms extends ctxt`,
   rw[ax_ctxt_def]
   \\ match_mp_tac extends_trans
-  \\ qspec_then`tys`(part_match_exists_tac(last o strip_conj) o concl o UNDISCH)NewTypes_ctxt_extends_hol_ctxt
-  \\ simp[NewTypes_ctxt_extends_hol_ctxt]
+  \\ qspec_then`tys`(part_match_exists_tac(last o strip_conj) o concl o UNDISCH)NewTypes_ctxt_extends
+  \\ simp[NewTypes_ctxt_extends]
+  \\ match_mp_tac extends_trans
+  \\ qpat_abbrev_tac`t = NewTypes_ctxt _ ++ _`
+  \\ qspecl_then[`t`,`tms`](part_match_exists_tac(last o strip_conj) o concl o UNDISCH)(Q.GEN`ctxt`NewConsts_ctxt_extends)
+  \\ dep_rewrite.DEP_REWRITE_TAC[NewConsts_ctxt_extends]
+  \\ simp[Abbr`t`]
   \\ REWRITE_TAC[GSYM APPEND_ASSOC]
-  \\ match_mp_tac NewConsts_ctxt_extends
-  \\ simp[]);
+  \\ match_mp_tac NewAxioms_ctxt_extends
+  \\ fs[]);
 
 val ax_tyass_def = xDefine"ax_tyass"`
-  ax_tyass0 ^mem select tys name args =
+  ax_tyass0 ^mem δ tys name args =
     case ALOOKUP tys name of
-    | NONE => tyaof (hol_model select (to_inner Ind)) name args
+    | NONE => δ name args
     | SOME (arity,cs) =>
       (case ALOOKUP cs args of
        | NONE => One
@@ -2750,17 +2794,13 @@ val _ = overload_on("ax_tyass",``ax_tyass0 ^mem``);
 
 val is_type_assignment_ax_tyass = Q.store_thm("is_type_assignment_ax_tyass",
   `is_set_theory ^mem ∧
-   good_select select ∧
-   wf_to_inner (to_inner Ind : ind -> 'U) ∧
+   is_type_assignment (tysof ctxt) δ ∧
    ^inhabited_tys
    ⇒
-   is_type_assignment (tysof (NewTypes_ctxt tys ++ hol_ctxt)) (ax_tyass select tys)`,
+   is_type_assignment (tysof (NewTypes_ctxt tys ++ ctxt)) (ax_tyass δ tys)`,
   rw[is_type_assignment_def,FEVERY_ALL_FLOOKUP,ALOOKUP_APPEND,ALOOKUP_type_list_NewTypes_ctxt]
   \\ rw[ax_tyass_def]
   \\ BasicProvers.TOP_CASE_TAC \\ fs[]
-  >- (
-    imp_res_tac hol_model_def
-    \\ fs[models_def,is_interpretation_def,is_type_assignment_def,FEVERY_ALL_FLOOKUP] )
   \\ split_pair_case_tac \\ fs[]
   \\ BasicProvers.CASE_TAC
   >- metis_tac[mem_one]
@@ -2775,7 +2815,7 @@ val ax_tyass_values = Q.store_thm("ax_tyass_values",
    EVERY
     (λ(name,arity,cs).
       EVERY
-        (λ(args,v). ax_tyass select tys name args = v)
+        (λ(args,v). ax_tyass δ tys name args = v)
         cs)
     tys`,
   rw[ax_tyass_def,EVERY_MEM]
@@ -2793,13 +2833,13 @@ val ax_tyass_values = Q.store_thm("ax_tyass_values",
   \\ res_tac \\ fs[]);
 
 val ax_tmass_def = xDefine"ax_tmass"`
-  ax_tmass0 ^mem select δ tms name args =
+  ax_tmass0 ^mem i tms name args =
   case ALOOKUP tms name of
-  | NONE => tmaof (hol_model select (to_inner Ind)) name args
+  | NONE => tmaof i name args
   | SOME (ty,cs) =>
     (case ALOOKUP cs args of
      | NONE =>
-       @u.  u <: typesem δ
+       @u.  u <: typesem (tyaof i)
                    ((K boolset) =++ ZIP(mlstring_sort (tyvars ty), args))
                    ty
      | SOME u => u)`;
@@ -2807,32 +2847,15 @@ val _ = overload_on("ax_tmass",``ax_tmass0 ^mem``);
 
 val is_term_assignment_ax_tmass = Q.store_thm("is_term_assignment_ax_tmass",
   `is_set_theory ^mem ∧
-   good_select select ∧
-   wf_to_inner (to_inner Ind : ind -> 'U) ∧
-   is_type_assignment (tysof ctxt) δ ∧
-   const_list ctxt = const_list hol_ctxt ∧
-   (∀name. name ∈ FDOM (tysof hol_ctxt) ⇒ δ name = tyaof (hol_model select (to_inner Ind)) name) ∧
+   is_term_assignment (tmsof ctxt) (tyaof i) (tmaof i) ∧
+   is_type_assignment (tysof ctxt) (tyaof i) ∧
    EVERY (type_ok (tysof ctxt) o FST o SND) tms ∧
-   EVERY (λ(name,ty,cs). EVERY (intype δ ty) cs) tms
+   EVERY (λ(name,ty,cs). EVERY (intype (tyaof i) ty) cs) tms
    ⇒
-   is_term_assignment (tmsof (NewConsts_ctxt tms ++ ctxt)) δ (ax_tmass select δ tms)`,
+   is_term_assignment (tmsof (NewConsts_ctxt tms ++ ctxt)) (tyaof i) (ax_tmass i tms)`,
   rw[is_term_assignment_def,FEVERY_ALL_FLOOKUP,ALOOKUP_APPEND,ALOOKUP_const_list_NewConsts_ctxt]
   \\ rw[ax_tmass_def]
   \\ BasicProvers.TOP_CASE_TAC \\ fs[]
-  >- (
-    imp_res_tac hol_model_def
-    \\ fs[models_def,is_interpretation_def,is_term_assignment_def,FEVERY_ALL_FLOOKUP]
-    \\ first_x_assum drule
-    \\ disch_then drule
-    \\ qmatch_abbrev_tac`_ <: m1 ⇒ _ <: m2`
-    \\ `m2 = m1` suffices_by rw[]
-    \\ unabbrev_all_tac
-    \\ match_mp_tac typesem_sig
-    \\ qexists_tac`tysof hol_ctxt`
-    \\ simp[]
-    \\ mp_tac theory_ok_hol_ctxt
-    \\ simp[theory_ok_def,IN_FRANGE_FLOOKUP,PULL_EXISTS]
-    \\ metis_tac[] )
   \\ split_pair_case_tac \\ fs[]
   \\ BasicProvers.CASE_TAC
   >- (
@@ -2907,7 +2930,7 @@ val ax_tmass_values = Q.store_thm("ax_tmass_values",
    EVERY
     (λ(name,ty,cs).
       EVERY
-        (λ(args,v). ax_tmass select δ tms name args = v)
+        (λ(args,v). ax_tmass i tms name args = v)
         cs)
     tms`,
   rw[ax_tmass_def,EVERY_MEM]
@@ -2925,30 +2948,49 @@ val ax_tmass_values = Q.store_thm("ax_tmass_values",
   \\ res_tac \\ fs[]);
 
 val ax_int_def = xDefine"ax_int"`
-  ax_int0 ^mem select tys tms =
-    (ax_tyass select tys,
-     ax_tmass select (ax_tyass select tys) tms)`;
+  ax_int0 ^mem i tys tms =
+    (ax_tyass (tyaof i) tys,
+     ax_tmass (ax_tyass (tyaof i) tys,tmaof i) tms)`;
 val _ = overload_on("ax_int",``ax_int0 ^mem``);
 
 val is_interpretation_ax_int = Q.store_thm("is_interpretation_ax_int",
   `is_set_theory ^mem ∧
-   good_select select ∧
-   wf_to_inner (to_inner Ind : ind -> 'U) ∧
+   theory_ok (thyof ctxt) ∧
+   is_interpretation (sigof ctxt) i ∧
    ^distinct_tys ∧
    ^inhabited_tys ∧
    ^types_ok ∧
-   EVERY (λ(name,ty,cs). EVERY (intype (ax_tyass select tys) ty) cs) tms
-   ⇒ is_interpretation (sigof (ax_ctxt tys tms)) (ax_int select tys tms)`,
+   EVERY (λ(name,ty,cs). EVERY (intype (ax_tyass (tyaof i) tys) ty) cs) tms
+   ⇒ is_interpretation (sigof (ax_ctxt ctxt ths tys tms)) (ax_int i tys tms)`,
   strip_tac
+  \\ qhdtm_x_assum`is_interpretation0`mp_tac
   \\ REWRITE_TAC[is_interpretation_def,ax_int_def,ax_ctxt_def]
-  \\ REWRITE_TAC[tysof_NewConsts_ctxt,GSYM APPEND_ASSOC]
+  \\ strip_tac
+  \\ REWRITE_TAC[tysof_NewAxioms_ctxt,tysof_NewConsts_ctxt,
+                 tmsof_NewAxioms_ctxt,GSYM APPEND_ASSOC]
+  \\ conj_asm1_tac
+  >- ( match_mp_tac is_type_assignment_ax_tyass \\ rw[] )
+  \\ qmatch_goalsub_abbrev_tac`(δ,γ):'U interpretation`
+  \\ `δ = tyaof (δ,γ)` by simp[]
+  \\ pop_assum(fn th => CONV_TAC(RATOR_CONV(ONCE_REWRITE_CONV[th])))
+  \\ match_mp_tac is_term_assignment_ax_tmass
+  \\ rw[] \\ fs[]
+  \\ fs[is_term_assignment_def,FEVERY_ALL_FLOOKUP]
+  \\ rw[]
+  \\ first_x_assum drule
+  \\ disch_then drule
+  \\ qmatch_abbrev_tac`_ <: t1 ⇒ _ <: t2`
+  \\ `t1 = t2` suffices_by rw[]
+  \\ unabbrev_all_tac
+  \\ match_mp_tac typesem_sig
+  \\ qexists_tac`tysof ctxt`
   \\ conj_asm1_tac
   >- (
-    match_mp_tac is_type_assignment_ax_tyass
-    \\ rw[] )
-  \\ match_mp_tac is_term_assignment_ax_tmass
-  \\ rw[]
-  \\ rw[FUN_EQ_THM,ax_tyass_def]
+    fs[theory_ok_def]
+    \\ first_x_assum match_mp_tac
+    \\ simp[IN_FRANGE_FLOOKUP]
+    \\ metis_tac[] )
+  \\ rw[ax_tyass_def,FUN_EQ_THM]
   \\ BasicProvers.CASE_TAC
   \\ imp_res_tac ALOOKUP_MEM
   \\ fs[ALL_DISTINCT_APPEND,MEM_MAP,PULL_EXISTS,EXISTS_PROD,MEM_type_list_NewTypes_ctxt]
@@ -2956,20 +2998,16 @@ val is_interpretation_ax_int = Q.store_thm("is_interpretation_ax_int",
 
 val is_std_interpretation_ax_int = Q.store_thm("is_std_interpretation_ax_int",
   `is_set_theory ^mem ∧
-   good_select select ∧
-   wf_to_inner (to_inner Ind : ind -> 'U) ∧
+   is_std_sig (sigof ctxt) ∧
+   is_std_interpretation i ∧
    ^distinct_tys ∧
    ^distinct_tms
    ⇒
-   is_std_interpretation (ax_int select tys tms)`,
+   is_std_interpretation (ax_int i tys tms)`,
   strip_tac
   \\ match_mp_tac (GEN_ALL is_std_interpretation_equal_on)
-  \\ qexists_tac`sigof hol_ctxt`
-  \\ qexists_tac`hol_model select (to_inner Ind)`
-  \\ imp_res_tac hol_model_def
-  \\ fs[models_def]
-  \\ reverse conj_tac
-  >- metis_tac[hol_is_bool_sig,is_bool_sig_std]
+  \\ qexists_tac`sigof ctxt`
+  \\ qexists_tac`i`
   \\ simp[equal_on_def,ax_int_def]
   \\ rw[ax_tyass_def,ax_tmass_def,FUN_EQ_THM]
   \\ BasicProvers.CASE_TAC
@@ -2980,22 +3018,24 @@ val is_std_interpretation_ax_int = Q.store_thm("is_std_interpretation_ax_int",
 
 val good_context_ax = Q.store_thm("good_context_ax",
   `is_set_theory ^mem ∧
-   good_select select ∧
-   wf_to_inner (to_inner Ind : ind -> 'U) ∧
+   theory_ok (thyof ctxt) ∧
+   is_interpretation (sigof ctxt) i ∧
+   is_std_interpretation i ∧
    ^distinct_tys ∧
    ^distinct_tms ∧
    ^inhabited_tys ∧
    ^types_ok ∧
-   EVERY (λ(name,ty,cs). EVERY (intype (ax_tyass select tys) ty) cs) tms
+   EVERY (λ(name,ty,cs). EVERY (intype (ax_tyass (tyaof i) tys) ty) cs) tms ∧
+   ^props_ok
    ⇒
-   good_context ^mem (sigof (ax_ctxt tys tms)) (ax_int select tys tms)`,
+   good_context ^mem (sigof (ax_ctxt ctxt ths tys tms)) (ax_int i tys tms)`,
   strip_tac
   \\ REWRITE_TAC[good_context_unpaired]
   \\ conj_tac >- first_assum ACCEPT_TAC
   \\ conj_tac
-  >- metis_tac[ax_ctxt_extends_hol_ctxt,is_std_sig_extends,hol_is_bool_sig,is_bool_sig_std]
+  >- metis_tac[ax_ctxt_extends_ctxt,is_std_sig_extends,theory_ok_sig,FST,SND]
   \\ conj_tac
   >- metis_tac[is_interpretation_ax_int]
-  \\ metis_tac[is_std_interpretation_ax_int]);
+  \\ metis_tac[is_std_interpretation_ax_int,theory_ok_sig,FST,SND]);
 
 val _ = export_theory()
